Baby's first high order functions

src/Utils.dfy
@@ -18,10 +18,29 @@ module Utils {
     }
 
     // what's monads, precious?
+    // also what's a standard library, precious? >:(
 
     function method Flatten<A>(ss: seq<seq<A>>) : seq<A>
     {
         if |ss| == 0 then [] else
         ss[0] + Flatten(ss[1..])
+    }
+
+    function method Map<T,U>(f: (T ~> U), s: seq<T>) : seq<U>
+        reads f.reads
+        requires forall i :: 0 <= i < |s| ==> f.requires(s[i])
+        ensures |s| == |Map(f, s)|
+    {
+        if |s| == 0 then [] else
+        [f(s[0])] + Map(f, s[1..])
+    }
+
+    function method Filter<T>(f: (T ~> bool), s: seq<T>) : seq<T>
+        reads f.reads
+        requires forall i :: 0 <= i < |s| ==> f.requires(s[i])
+        ensures |Filter(f, s)| <= |s|
+    {
+        if |s| == 0 then [] else
+        (if f(s[0]) then [s[0]] else []) + Filter(f, s[1..])
     }
 }
